newest/errorIFF.v
@@ -2,6 +2,7 @@ Require Import erasure.
 Require Import SpecImpliesNonSpec.
 Require Import stepWF. 
 Require Import IndependenceCommon.
+Require Import nonspeculativeImpliesSpeculative. 
 
 Theorem raw_eraseFull : forall H x N tid ds,
                           raw_heap_lookup x H = Some(sfull COMMIT ds COMMIT tid N) ->
@@ -36,128 +37,15 @@ Proof.
   erewrite <- decomposeErase in H1; eauto. simpl. auto. eauto. 
 Qed. 
 
-Theorem lookupSomeUnique : forall T H x v S,
-                             unique T S H -> Ensembles.In AST.id S x ->
-                             raw_heap_lookup x H = Some v -> False. 
+Theorem ParErrorSpecError : forall H T t H' T' t',
+                              pstep H T t pError -> specHeap H H' -> speculate T T' ->
+                              speculate t t' -> multistep H' (tUnion T' t') None.  
 Proof.
-  induction H; intros. 
-  {inv H1. }
-  {simpl in *. destruct a. destruct (beq_nat x i) eqn:eq. 
-   {inv H2. inv H0. apply beq_nat_true in eq. subst. contradiction. }
-   {inv H0. eapply IHlist; eauto. constructor. auto. }
-  }
-Qed. 
-
-Theorem raw_eraseFull' : forall H x N S, 
-          unique ivar_state S H ->
-          raw_heap_lookup x (raw_eraseHeap H) = Some(pfull (eraseTerm N)) ->
-          exists tid ds, raw_heap_lookup x H = 
-                         Some(sfull COMMIT ds COMMIT tid N). 
-Proof.
-  induction H; intros. 
-  {inv H0. } 
-  {simpl in *. destruct a. destruct (beq_nat x i) eqn:eq. 
-   {destruct i0. destruct s. inv H0. eapply IHlist in H1; eauto. 
-    invertHyp. eapply lookupSomeUnique in H1; eauto. inv H1. apply beq_nat_true in eq. 
-    subst. apply Ensembles.Union_intror. constructor. simpl in *. rewrite eq in H1. inv H1. 
-    destruct s. eapply IHlist in H1. invertHyp. inv H0. eapply lookupSomeUnique in H1; eauto. 
-    contradiction. apply beq_nat_true in eq. subst. apply Ensembles.Union_intror. constructor. 
-    inv H0. eauto. destruct s0. simpl in H1. rewrite eq in H1. inv H1. simpl in *. 
-    rewrite eq in H1. inv H1. apply eraseTermUnique in H3. subst. eauto. }
-   {destruct i0. destruct s; inv H0; eauto. simpl in H1. rewrite eq in H1. 
-    eauto. destruct s. inv H0; eauto. destruct s0. simpl in *. rewrite eq in H1.
-    inv H0; eauto. simpl in *. rewrite eq in H1. inv H0. eauto. }
-  }
-Qed. 
-
-
-Theorem eraseFull' : forall H x N, 
-                       heap_lookup x (eraseHeap H) = Some(pfull (eraseTerm N)) ->
-                       exists tid ds, heap_lookup x H = Some(sfull COMMIT ds COMMIT tid N). 
-Proof.
-  intros. destruct H. simpl in *. eapply raw_eraseFull' in H0; eauto. 
-Qed. 
-
-Ltac invertActList :=
-  match goal with
-      |H:aCons ?A ?b = locked nil |- _ => destruct b; inv H
-      |H:aCons ?A ?b = unlocked nil |- _ => destruct b; inv H
-  end. 
-
-Theorem spec_multi_false : forall T T' tid s1 x M' E N d s2 M H H' a b c,
-                             spec_multistep H (tUnion T (tSingleton(tid,unlocked nil,s2,M'))) H'
-                                            (tUnion T' (tSingleton(tid,unlocked(s1++[wAct x M' E N d]),s2,M))) ->
-                             heap_lookup x H = Some(sfull COMMIT a COMMIT b c) ->
-                             False. 
-Proof.
-  intros. genDeps{a; b; c}. dependent induction H0; intros.
-  {subst. apply UnionEqTID in x. invertHyp. inv H. invertListNeq. }
-  {startIndCase. destructThread x1. exMid tid H7. 
-   {apply UnionEqTID in x. invertHyp. inv H; try solve[falseDecomp]. 
-    {inv H13; falseDecomp. }
-    {copy d; copy d0. eapply uniqueCtxtDecomp in H; eauto. invertHyp. inv H5. 
-     heapsDisagree. }
-   }
-   {apply UnionNeqTID in x. invertHyp. eapply specStepFullIVar in H; eauto. 
-    invertHyp. eapply IHspec_multistep; eauto. rewrite H2. unfoldTac. 
-    rewrite UnionSwap. eauto. auto. }
-  }
-Qed. 
-
-Theorem wfDoubleWrite : forall H T tid s1' x M' E N d s2 M a b c,
-                          wellFormed H (tAdd T (tid,unlocked(s1'++[wAct x M' E N d]),s2,M)) ->
-                          heap_lookup x H = Some(sfull COMMIT a COMMIT b c) -> False. 
-Proof.
-  intros. inv H0. unfoldTac. rewrite AddUnion in H3. rewrite unspecUnionComm in H3. 
-  erewrite unspecLastActPool in H3. Focus 2. constructor. eapply spec_multi_false in H3. 
-  auto. eapply unspecHeapLookupFull; eauto. 
-Qed. 
-
-
-Theorem commitPoolUnionComm : forall T1 T2, 
-                                commitPool (tUnion T1 T2) -> 
-                                commitPool T1 /\ commitPool T2. 
-Proof.
-  induction T2; intros. 
-  {simpl in *. unfoldTac. rewrite union_empty_r in H. auto. }
-  {destructThread a. destruct H5. 
-   {unfoldTac. rewrite Union_commutative in H. simpl in *. contradiction. }
-   {destruct l. 
-    {simpl. apply IHT2. unfoldTac. rewrite Union_commutative in H. simpl in H. 
-     rewrite Union_commutative. auto. }
-    {unfoldTac. rewrite Union_commutative in H. simpl in *. contradiction. }
-   }
-   {unfoldTac. rewrite Union_commutative in H. simpl in *. contradiction. }
-  }
-Qed. 
-
-Theorem commitEraseSingle : forall t t',
-                              commitPool t -> erasePool t = pSingle t' ->
-                              exists tid s2 M, t = tSingleton(tid,unlocked nil, s2, M) /\
-                                               eraseTerm M = t'. 
-Proof.
-  intros. destruct t. 
-  {inv H0. }
-  {destructThread t. destruct H6; try contradiction.  
-   destruct l; try contradiction. simpl in *. destruct t0. 
-   {inv H0. econstructor. econstructor. econstructor. split; eauto. unfold tSingleton.
-    unfold Single. reflexivity. }
-   {inv H0. destructThread t. destruct H9; try contradiction. destruct l; try contradiction. 
-    simpl in *. inv H6. }
-  }
-Qed. 
-
-Theorem ParErrorSpecError : forall H T t,
-                               wellFormed H (tUnion T t) -> commitPool (tUnion T t) ->
-                               pstep (eraseHeap H) (erasePool T) (erasePool t) pError ->
-                               multistep H (tUnion T t) None. 
-Proof.
-  intros. inv H2. 
-  {existTac E. existTac N. existTac M. apply commitPoolUnionComm in H1. invertHyp.
-   eapply commitEraseSingle in H5; eauto. invertHyp. simpl in *. 
-   rewrite decomposeErase with(e:=put (fvar x) x2)in H4; eauto. apply eraseFull' in H7.
-   invertHyp. eapply smulti_error. econstructor; eauto. }
-Qed. 
+  intros. inv H0. inv H3. inv H7. copy H4. apply decomposeSpec in H4. 
+  unfoldTac. eapply specHeapLookupFull in H5; eauto. invertHyp. 
+  rewrite Union_associative. eapply Spec.smulti_error. eapply ErrorWrite. 
+  simpl in *. eauto. eauto. 
+Qed.                          
  
 Theorem pmulti_trans : forall H T H' T' c, 
                          pmultistep H T (Some(H', T')) ->
@@ -182,14 +70,26 @@ Proof.
    eapply pmulti_error. eauto. }
 Qed. 
 
-
-Theorem ParErrorSpecErrorStar : forall H T,
-                                  wellFormed H T -> commitPool T -> 
-                                  pmultistep (eraseHeap H) (erasePool T) None -> 
-                                  multistep H T None. 
+Theorem multi_trans : forall H T H' T' c, multistep H T (Some(H', T')) ->  
+                                          multistep H' T' c ->
+                                          multistep H T c. 
 Proof.
-  Admitted. (*This needs ParImpliesSpec first*)
+  intros. remember (Some(H',T')). induction H0. 
+  {inv Heqo. auto. }
+  {subst. econstructor. eauto. eauto. }
+  {inv Heqo. }
+Qed. 
 
+Theorem ParErrorSpecErrorStar : forall H T H' T',
+                                  pmultistep H T None -> specHeap H H' -> heapWF H -> PoolWF T ->
+                                  speculate T T' -> multistep H' T' None. 
+Proof.
+  intros. genDeps{H'; T'}. dependent induction H0; intros. 
+  {copy H0. eapply nonspecImpliesSpec in H0; eauto. invertHyp. 
+   eapply pstepWF in H6; eauto. invertHyp. inv H7. econstructor. 
+   eauto. eapply multi_trans. eassumption. eapply IHpmultistep; eauto. }
+  {apply specUnionComm in H4. invertHyp. eapply ParErrorSpecError in H0; eauto. }
+Qed. 
 
 
 
