newest/nonspecImpliesCommitStep.v
@@ -1,0 +1,150 @@
+Require Import erasure. 
+Require Import IndependenceCommon. 
+Require Import stepWF. 
+Require Import nonspeculativeImpliesSpeculative. 
+
+Inductive prog_multistep : sHeap -> pool -> option (sHeap * pool) -> Prop :=
+|prog_multi_refl : forall H T, prog_multistep H T (Some (H, T))
+|prog_multi_step : forall H H' c T t t',
+                prog_step H T t (OK H' T t') -> prog_multistep H' (tUnion T t') c ->
+                prog_multistep H (tUnion T t) c
+|prog_smulti_error : forall H T t, 
+                  prog_step H T t Error -> prog_multistep H (tUnion T t) None. 
+
+Inductive stepPlus : sHeap -> pool -> option (sHeap * pool) -> Prop :=
+| plus_step : forall (H H' : sHeap) c (T t t' : pool),
+                 prog_step H T t (OK H' T t') ->
+                 prog_multistep H' (tUnion T t') c -> stepPlus H (tUnion T t) c
+| plus_error : forall (H : sHeap) (T t : pool),
+                   prog_step H T t Spec.Error -> stepPlus H (tUnion T t) None.
+
+Theorem nonspecImpliesSpec : forall PH PH' PT pt pt' T H,
+        pstep PH PT pt (pOK PH' PT pt') -> 
+        speculate (pUnion PT pt) T -> PoolWF (pUnion PT pt) -> heapWF PH -> specHeap PH H ->
+        exists T' H', stepPlus H T (Some(H', T')) /\
+                   speculate (pUnion PT pt') T' /\ specHeap PH' H'. 
+Proof.
+  intros. inv H0. 
+  {apply specUnionComm in H1. invertHyp. inv H1. inv H7. econstructor. econstructor. 
+   split. unfoldTac. rewrite Union_associative. econstructor. 
+   eapply simBasicStep in H9. eapply CBasicStep. eauto. constructor. split; auto. 
+   apply poolWFComm in H2. simpl in H2. invertHyp. eapply basicStepGather in H9; eauto. 
+   unfoldTac. rewrite <- Union_associative. apply specUnionComm'. auto. 
+   constructor. constructor. auto. }
+  {copy H9. apply specUnionComm in H1. invertHyp. inv H1. inv H8.
+   eapply gatherDecomp in H0; eauto. invertHyp. econstructor. econstructor. split. 
+   unfoldTac. rewrite Union_associative. econstructor.
+   eapply CSpec with(M:=specTerm M)(N:=specTerm N)(E:=specCtxt E). 
+   eapply multi_step. eapply PopSpec. rewrite app_nil_l. simpl. auto. constructor. 
+   split. unfoldTac. rewrite <- Union_associative. apply specUnionComm'. auto.
+   rewrite couple_swap. rewrite coupleUnion. repeat rewrite Union_associative. 
+   replace (specRun(specTerm M)(specTerm N)) with (specTerm(pspecRun M N)); auto.  
+   rewrite <- specFill. constructor. constructor. rewrite <- Union_associative. 
+   apply gatherFill; auto. inv H0. constructor; auto. auto. }
+  {copy H9. apply specUnionComm in H1. invertHyp. inv H1. inv H8. 
+   eapply gatherDecomp in H0; eauto. invertHyp. inv H0. unfoldTac. 
+   repeat rewrite <- Union_associative. rewrite listToSingle. rewrite <- coupleUnion. 
+   rewrite couple_swap. repeat rewrite Union_associative. econstructor. econstructor. split.
+   econstructor. eapply SpecJoin with (N0:=specTerm M)
+                          (M:=specTerm M)(N1:=specTerm N)(E:=specCtxt E); eauto. 
+   simpl. constructor. split. unfoldTac. repeat rewrite <- Union_associative. apply specUnionComm'. 
+   auto. rewrite (Union_associative thread x0).
+   rewrite (Union_associative thread (Union thread x0 T1)). 
+   replace (specJoin(ret(specTerm N)) (specTerm M)) with (specTerm (pspecJoin (pret N) M)); auto. 
+   rewrite <- specFill. constructor. constructor. rewrite <- Union_associative. 
+   apply gatherFill. auto. constructor; auto. auto. }
+  {copy H9. apply specUnionComm in H1. invertHyp. inv H1. inv H8. 
+   eapply gatherDecomp in H0; eauto. invertHyp. inv H0. unfoldTac. 
+   repeat rewrite <- Union_associative. rewrite listToSingle. rewrite <- coupleUnion. 
+   repeat rewrite Union_associative. rewrite <- Union_associative. econstructor. econstructor. split.  
+   econstructor. apply decomposeSpec in H9.
+   eapply SpecRB with (E:=specTerm N)(E':=specCtxt E)(N0:=specTerm M). eassumption. 
+   auto. auto. eapply RBDone. unfold tAdd. unfold Add. unfoldTac. unfold In. 
+   apply in_app_iff. right. simpl. left; eauto. eauto.
+   constructor. split. unfoldTac. repeat rewrite <- Union_associative. apply specUnionComm'. 
+   auto. replace (raise (specTerm N)) with (specTerm (praise N)); auto. rewrite <- specFill.
+   apply gatherSourceProg in H12. Focus 2. apply poolWFComm in H2. simpl in H2. invertHyp.
+   apply ptrmDecomposeWF in H9; auto. inv H9. auto. subst. unfold Add. simpl. 
+   rewrite Union_associative. constructor. constructor. apply gatherFill; auto. auto. }
+  {copy H9. apply specUnionComm in H1. invertHyp. inv H1. inv H8. 
+   eapply gatherDecomp in H0; eauto. invertHyp. inv H0. copy H9. rewrite poolWFComm in H2. 
+   simpl in H2. invertHyp. apply ptrmDecomposeWF in H9; auto. simpl in H9. 
+   unfoldTac. rewrite Union_associative. econstructor. econstructor. split. econstructor. 
+   eapply Fork with (M:=specTerm M)(E:=specCtxt E). eauto. eapply multi_step. eapply PopFork. 
+   rewrite app_nil_l. simpl. auto. auto. constructor. unfoldTac. rewrite <- Union_associative. 
+   split. apply specUnionComm'. auto. copy H7. apply gatherSourceProg in H7; auto. rewrite H7. 
+   rewrite union_empty_r. rewrite coupleUnion. unfold pCouple. unfold Couple. simpl. 
+   replace (ret unit) with (specTerm (pret punit)); auto. rewrite <- specFill. constructor. 
+   rewrite <- union_empty_l. constructor. constructor. subst. eauto. 
+   rewrite <- union_empty_r. apply gatherFill. auto. repeat constructor. auto. }
+  {copy H11. apply specUnionComm in H1. invertHyp. inv H1. inv H8. copy H10. 
+   eapply specHeapLookupFull in H10; eauto. invertHyp. 
+   eapply gatherDecomp in H0; eauto. invertHyp. 
+   econstructor. econstructor. split. unfoldTac. rewrite Union_associative. econstructor. 
+   eapply Get with (N:=specTerm M)(E:=specCtxt E). eauto. auto. eapply multi_step. eapply PopRead. 
+   rewrite app_nil_l. simpl; auto. rewrite app_nil_r. rewrite app_nil_l. auto. introsInv. 
+   erewrite HeapLookupReplace; eauto. auto. rewrite replaceOverwrite. rewrite replaceSame. 
+   constructor. eauto. unfoldTac. rewrite Union_associative. repeat rewrite <- Union_associative. 
+   split. apply specUnionComm'. auto. inv H0. inv H9. simpl. 
+   replace (ret(specTerm M)) with (specTerm(pret M)); auto. rewrite <- specFill. 
+   constructor. constructor. rewrite <- union_empty_r. apply gatherFill. auto. constructor.
+   gatherTac M. copy H8. apply gatherSourceProg in H8; eauto. subst. auto. Focus 2. auto.
+   eapply lookupSourceProg; eauto. } 
+  {apply specUnionComm in H1. invertHyp. inv H1. inv H8. copy H7. 
+   eapply gatherDecomp in H7; eauto. invertHyp. rewrite poolWFComm in H2. simpl in H2. 
+   invertHyp. econstructor. econstructor. split. unfoldTac. rewrite Union_associative. 
+   econstructor. eapply Put with (N:=specTerm M)(E:=specCtxt E).
+   simpl in *. eauto. eapply specHeapLookupEmpty; eauto. auto. eapply multi_step. 
+   eapply PopWrite. rewrite app_nil_l. simpl; auto. erewrite HeapLookupReplace; eauto. 
+   eapply specHeapLookupEmpty; eauto. auto. rewrite replaceOverwrite. constructor. 
+   split. unfoldTac. rewrite <- Union_associative. apply specUnionComm'. auto. 
+   inv H6. inv H13. unfoldTac. simpl in *. copy H1. apply ptrmDecomposeWF in H6; auto. inv H6. 
+   eapply gatherSourceProg in H15; eauto. subst. rewrite union_empty_r in *.  
+   replace (ret unit) with (specTerm (pret punit)); auto. rewrite <- specFill. constructor. 
+   constructor. rewrite <- union_empty_r. apply gatherFill. auto. repeat constructor. 
+   apply specHeapReplaceFull; auto. }
+  {apply specUnionComm in H1. invertHyp. inv H1. inv H7. copy H10. 
+   eapply gatherDecomp in H10; eauto. invertHyp. rewrite poolWFComm in H2. simpl in H2. 
+   invertHyp. econstructor. econstructor. split. unfoldTac. rewrite Union_associative. 
+   econstructor. copy p. eapply specHeapLookupNone in H8; eauto.
+   eapply New with (E:=specCtxt E)(x:=x). auto. eapply multi_step. 
+   eapply PopNewEmpty.  rewrite app_nil_l. simpl; auto. rewrite lookupExtend. auto. 
+   auto. erewrite replaceExtendOverwrite; eauto. constructor. unfoldTac.
+   rewrite <- Union_associative. apply specUnionComm'. auto. 
+   replace (ret(fvar x)) with (specTerm(pret(pfvar x))); auto. rewrite <- specFill. 
+   constructor. constructor. apply gatherFill; auto. constructor. inv H6. constructor. 
+   apply specHeapExtend; auto. }
+  Grab Existential Variables. 
+  {eapply specHeapLookupNone; eauto. }
+  {apply decomposeSpec in H1. auto. }
+  {eapply specHeapLookupNone; eauto. }
+  {apply decomposeSpec in H1; auto. }
+  {apply decomposeSpec in H11. auto. }
+  {apply decomposeSpec in H0. auto. }
+  {apply decomposeSpec in H9; auto. }
+  {apply decomposeSpec in H9; auto. }
+Qed. 
+
+Theorem nonspecImpliesSpecStar : forall PH PH' PT H PT' T,
+        pmultistep PH PT (Some(PH', PT')) -> 
+        speculate PT T -> PoolWF PT -> heapWF PH -> specHeap PH H ->
+        exists T' H', multistep H T (Some(H', T')) /\
+                   speculate PT' T' /\ specHeap PH' H'. 
+Proof.
+  intros. remember (Some(PH',PT')). genDeps{H; T}. induction H0; intros.  
+  {inv Heqo. eauto. }
+  {intros. subst. copy H0. eapply nonspecImpliesSpec in H0; eauto. invertHyp.
+   copy H7. apply pstepWF in H7; auto. invertHyp. 
+   eapply IHpmultistep in H10; eauto. invertHyp. econstructor. econstructor. split.
+   inv H8. eapply multi_step. eauto. eapply multi_trans; eauto. eauto. }
+  {inv Heqo. }
+Qed. 
+
+
+
+
+
+
+
+
+
