newest/nonspecPar.v
@@ -1,0 +1,375 @@
+Require Export AST.   
+Require Export Heap.
+Require Export sets. 
+Require Export Coq.Program.Equality.
+Require Export multiset. 
+Require Import NonSpec. 
+
+(*Syntax for non-speculative Par Monad semantics (uses locally nameless cofinite quantification*)
+Inductive ptrm' : Type :=
+|pfvar' : id -> ptrm'
+|pbvar' : id -> ptrm'
+|punit' : ptrm'
+|ppair' : ptrm' -> ptrm' -> ptrm'
+|plambda' : ptrm' -> ptrm'
+|papp' : ptrm' -> ptrm' -> ptrm'
+|pret' : ptrm' -> ptrm'
+|pbind' : ptrm' -> ptrm' -> ptrm'
+|pfork' : ptrm' -> ptrm'
+|pnew' : ptrm'
+|pput' : ptrm' -> ptrm' -> ptrm'
+|pget' : ptrm' -> ptrm'
+|praise' : ptrm' -> ptrm'
+|phandle' : ptrm' -> ptrm' -> ptrm'
+|pfst' : ptrm' -> ptrm'
+|psnd' : ptrm' -> ptrm'
+|pdone' : ptrm' -> ptrm'
+.
+
+Fixpoint popen' (k:nat) (u:ptrm') (t:ptrm') : ptrm' :=
+  match t with
+      |pbvar' i => if beq_nat k i then u else t
+      |ppair' e1 e2 => ppair' (popen' k u e1) (popen' k u e2)
+      |plambda' e => plambda' (popen'  (S k) u e)
+      |papp' e1 e2 => papp' (popen' k u e1) (popen' k u e2)
+      |pret' e => pret' (popen' k u e)
+      |pbind' e1 e2 => pbind' (popen' k u e1) (popen' k u e2)
+      |pfork' e => pfork' (popen' k u e)
+      |pput' i e => pput' (popen' k u i) (popen' k u e)
+      |pget' i => pget' (popen' k u i)
+      |praise' e => praise' (popen' k u e)
+      |phandle' e1 e2 => phandle' (popen' k u e1) (popen' k u e2)
+      |pfst' e => pfst' (popen' k u e)
+      |psnd' e => psnd' (popen' k u e)
+      |pdone' e => pdone' (popen' k u e)
+      |_ => t
+  end. 
+
+Inductive pivar_state' : Type :=
+|pempty' : pivar_state'
+|pfull' : ptrm' -> pivar_state'.
+
+Definition pHeap' := heap pivar_state'. 
+
+Inductive pctxt' : Type :=
+|pbindCtxt : pctxt' -> ptrm' -> pctxt'
+|phandleCtxt : pctxt' -> ptrm' -> pctxt'
+|pappctxt' : pctxt' -> ptrm' -> pctxt' 
+|pappValCtxt : pctxt' -> ptrm' -> pctxt'
+|ppairCtxt : pctxt' -> ptrm' -> pctxt'
+|ppairValCtxt : pctxt' -> ptrm' -> pctxt'
+|pfstCtxt : pctxt' -> pctxt' 
+|psndCtxt : pctxt' -> pctxt'  
+|pholeCtxt : pctxt'
+.
+
+Inductive pval' : ptrm' -> Prop :=
+|pretVal' : forall M, pval' (pret' M)
+|praiseVal' : forall M, pval' (praise' M)
+|plamVal' : forall M, pval' (plambda' M)
+|ppairVal' : forall M N, pval' M -> pval' N -> pval' (ppair' M N).
+
+Inductive pdecompose' : ptrm' -> pctxt' -> ptrm' -> Prop :=
+|pdecompBind : forall M N E M', ~ pval' M -> pdecompose' M E M' ->
+                                pdecompose' (pbind' M N) (pbindCtxt E N) M'
+|pdecompBindVal : forall M N, pval' M ->
+                              pdecompose' (pbind' M N) pholeCtxt (pbind' M N)
+|pdecompHandle : forall M M' N E, ~pval' M -> pdecompose' M E M' -> pdecompose' (phandle' M N) (phandleCtxt E N) M'
+|pdecompHandleVal : forall M N, pval' M -> pdecompose' (phandle' M N) pholeCtxt (phandle' M N)
+|pdecompApp : forall M N M' E, ~pval' M -> pdecompose' M E M' -> pdecompose' (papp' M N) (pappctxt' E N) M'
+|pdecompAppVal1 : forall M N N' E, pval' M -> ~pval' N -> pdecompose' N E N' ->
+                                   pdecompose' (papp' M N) (pappValCtxt E M) N'
+|pdecompAppVal2 : forall M N, pval' M -> pval' N -> pdecompose' (papp' M N) pholeCtxt (papp' M N)
+|pdecompFst : forall M E M', ~pval' M -> pdecompose' M E M' -> pdecompose' (pfst' M) (pfstCtxt E) M'
+|pdecompFstVal : forall M, pval' M -> pdecompose' (pfst' M) pholeCtxt (pfst' M)
+|pdecompSnd : forall M E M', ~pval' M -> pdecompose' M E M' -> pdecompose' (psnd' M) (psndCtxt E) M'
+|pdecompSndVal : forall M, pval' M -> pdecompose' (psnd' M) pholeCtxt (psnd' M)
+|pdecompNew : pdecompose' pnew' pholeCtxt pnew'
+|pdecompGet : forall i, pdecompose' (pget' i) pholeCtxt (pget' i)
+|pdecompPut : forall i M, pdecompose' (pput' i M) pholeCtxt (pput' i M)
+|pdecompFork : forall M, pdecompose' (pfork' M) pholeCtxt (pfork' M)
+|pdecompPair : forall M M' E N, ~pval' M -> pdecompose' M E M' ->
+                                pdecompose' (ppair' M N) (ppairCtxt E N) M'
+|pdecompPairVal : forall M N N' E, pval' M -> ~pval' N -> pdecompose' N E N' ->
+                                   pdecompose' (ppair' M N) (ppairValCtxt E M) N'
+.  
+
+Fixpoint pfill' (c:pctxt') (t:ptrm') : ptrm' :=
+  match c with
+      |pbindCtxt E N => pbind' (pfill' E t) N
+      |phandleCtxt E N => phandle' (pfill' E t) N
+      |pappctxt' E N => papp' (pfill' E t) N
+      |pappValCtxt E M => papp' M (pfill' E t)
+      |ppairCtxt E N => ppair' (pfill' E t) N
+      |ppairValCtxt E M => ppair' M (pfill' E t)
+      |pfstCtxt E => pfst' (pfill' E t)
+      |psndCtxt E => psnd' (pfill' E t)
+      |pholeCtxt => t
+  end. 
+
+Ltac helperTac :=
+  match goal with
+    |H:?x=?y |- _ => inversion H; subst; clear H
+    |H:forall M e, (?x,?y) = (M, e) -> ?z |- _ => assert(EQ:(x,y)=(x,y)) by auto; apply H in EQ
+  end. 
+
+Theorem pdecompose'Eq : forall M E e, pdecompose' M E e -> M = pfill' E e. 
+Proof.
+  induction M; intros; try solve[inversion H; subst; auto]; 
+  try solve[inversion H; subst; auto; simpl; apply IHM1 in H5; subst; auto].
+  {inversion H; subst. apply IHM1 in H5. subst. auto. apply IHM2 in H6. subst. auto. }
+  {inversion H; subst. apply IHM1 in H5; subst; auto. apply IHM2 in H6; subst; auto. auto. }
+  {inversion H; subst; auto. apply IHM in H2; subst; auto. }
+  {inversion H; subst; auto. apply IHM in H2; subst; auto. }
+Qed. 
+
+Ltac inv H := inversion H; subst; clear H.
+
+Theorem pctxt'Unique : forall M E E' e e', pdecompose' M E e -> pdecompose' M E' e' ->
+                                          E = E' /\ e = e'. 
+Proof.
+  induction M; intros; try solve[inversion H; inversion H0; subst; auto]. 
+  {inv H; inv H0; try contradiction. eapply IHM1 in H6; eauto. inv H6. auto.  
+   eapply IHM2 in H7; eauto. inv H7; auto. }
+  {inv H; inv H0; try contradiction. eapply IHM1 in H6; eauto. inv H6; auto. 
+   eapply IHM2 in H7; eauto. inv H7; auto. auto. }
+  {inv H; inv H0; try contradiction. eapply IHM1 in H6; eauto. inv H6; auto. auto. }
+  {inv H; inv H0; try contradiction; auto. eapply IHM1 in H6; eauto. inv H6; auto. }
+  {inv H; inv H0; try contradiction; auto. eapply IHM in H3; eauto. inv H3; auto. }
+  {inv H; inv H0; try contradiction; auto. eapply IHM in H3; eauto. inv H3; auto. }
+Qed. 
+
+Definition pPool' := multiset ptrm'. 
+Definition pSingle' := Single ptrm'. 
+Definition pUnion' := Union ptrm'. 
+Definition pCouple' := Couple ptrm'. 
+
+Inductive pconfig' : Type :=
+|pError' : pconfig'
+|pOK' : pHeap' -> pPool' -> pPool' -> pconfig'. 
+
+Inductive pbasic_step : ptrm' -> ptrm' -> Prop :=
+|pbasicBeta : forall t E e N,  pdecompose' t E (papp'(plambda' e) N) ->
+                              pbasic_step t (pfill' E (popen' 0 N e))
+|pbasicProjL : forall t E V1 V2,
+                pdecompose' t E (pfst' (ppair' V1 V2)) -> pbasic_step t (pfill' E V1)
+|pbasicProjR : forall t E V1 V2,
+                pdecompose' t E (psnd'(ppair' V1 V2)) -> pbasic_step t (pfill' E V2)
+|pbasicBind : forall t E M N,
+               pdecompose' t E (pbind' (pret' M) N) -> pbasic_step t (pfill' E (papp' N M))
+|pbasicBindRaise : forall t E M N,
+                    pdecompose' t E (pbind' (praise' M) N) -> pbasic_step t (pfill' E (praise' M))
+|pbasicHandle : forall t E M N,
+                 pdecompose' t E (phandle' (praise' M) N) -> pbasic_step t (pfill' E (papp' N M))
+|pbasicHandleRet : forall t E M N,
+                    pdecompose' t E (phandle' (pret' M) N) -> pbasic_step t (pfill' E (pret' M)). 
+
+Inductive pstep' : pHeap' -> pPool' -> pPool' -> pconfig' -> Prop :=
+|PBasicStep : forall t t' h T,
+                pbasic_step t t' -> pstep' h T (pSingle' t) (pOK' h T (pSingle' t'))
+|pFork : forall E t M h T,
+           pdecompose' t E (pfork' M) -> 
+           pstep' h T (pSingle' t) (pOK' h T (pCouple' (pfill' E(pret' punit')) M))
+|PGet : forall E M t h T x,
+           heap_lookup x h = Some(pfull' M) -> pdecompose' t E (pget' (pfvar' x)) -> 
+           pstep' h T (pSingle' t) (pOK' h T (pSingle' (pfill' E(pret' M))))
+|PPut : forall E t M h h' T x,
+          pdecompose' t E (pput' (pfvar' x) M) -> heap_lookup x h = Some pempty' ->
+          h' = replace x (pfull' M) h ->
+          pstep' h T (pSingle' t) (pOK' h' T (pSingle' (pfill' E (pret' punit'))))
+|PPutError : forall E t M h T x N,
+               pdecompose' t E (pput' (pfvar' x) M) -> heap_lookup x h = Some (pfull' N) ->
+               pstep' h T (pSingle' t) pError'
+|PNew : forall E t h h' T x (p:heap_lookup x h = None),
+          pdecompose' t E pnew' ->  h' = extend x pempty' h p ->
+          pstep' h T (pSingle' t) (pOK' h' T (pSingle' (pfill' E (pret' (pfvar' x)))))
+.
+
+Inductive pmultistep' : pHeap' -> pPool' -> option (pHeap' * pPool') -> Prop :=
+|pmulti_refl' : forall H T, pmultistep' H T (Some (H, T))
+|pmulti_step' : forall H H' T t t' c,
+                 pstep' H T t (pOK' H' T t') -> pmultistep' H' (pUnion' T t') c ->
+                 pmultistep' H (pUnion' T t) c
+|pmulti_error' : forall H T t,
+                  pstep' H T t pError' -> 
+                  pmultistep' H (pUnion' T t) None.    
+
+Ltac depInd H := generalize_eqs_vars H; induction H; simplify_dep_elim; intros.
+
+Theorem pmulti_trans : forall H T H' T' H'' T'',
+                         pmultistep' H T (Some (H', T')) -> 
+                         pmultistep' H' T' (Some (H'', T'')) ->
+                         pmultistep' H T (Some (H'', T'')).
+Proof.
+  intros. depInd H0. 
+  {auto. }
+  {econstructor; eauto. }
+Qed. 
+
+Inductive pctxt'WF (e:ptrm') : pctxt' -> Prop :=
+|pbindWF : forall N E, pctxt'WF e E -> ~pval' (pfill' E e) -> pctxt'WF e (pbindCtxt E N)
+|phandleWF : forall N E, pctxt'WF e E -> ~pval' (pfill' E e) -> pctxt'WF e (phandleCtxt E N)
+|pappWF : forall N E, pctxt'WF e E -> ~pval' (pfill' E e) -> pctxt'WF e (pappctxt' E N)
+|pappValWF : forall M E, pctxt'WF e E -> pval' M -> ~pval' (pfill' E e) -> pctxt'WF e (pappValCtxt E M)
+|ppairWF : forall N E, pctxt'WF e E -> ~pval' (pfill' E e) -> pctxt'WF e (ppairCtxt E N)
+|ppairValWF : forall M E, pctxt'WF e E -> pval' M -> ~pval' (pfill' E e) -> pctxt'WF e (ppairValCtxt E M)
+|pfstWF : forall E, pctxt'WF e E -> ~pval' (pfill' E e) -> pctxt'WF e (pfstCtxt E)
+|psndWF : forall E, pctxt'WF e E -> ~pval' (pfill' E e) -> pctxt'WF e (psndCtxt E)
+|pholEWF : pctxt'WF e pholeCtxt. 
+
+Theorem pdecompose'Decomposed : forall E e, pctxt'WF e E ->
+                                          pdecompose' e pholeCtxt e -> 
+                                          pdecompose' (pfill' E e) E e. 
+Proof.
+  intros. induction H; try solve[simpl; constructor; auto]. 
+  {simpl. assumption. }
+Qed. 
+
+Hint Constructors pctxt'WF. 
+
+Ltac copy H :=
+  match type of H with
+      |?x => assert(x) by auto
+  end. 
+
+Theorem pdecompose'WF : forall t E e, pdecompose' t E e -> pctxt'WF e E. 
+Proof.
+  induction t; intros; try solve[inversion H];
+  try solve[inversion H; subst; auto; copy H5; apply IHt1 in H5; constructor; auto; 
+   apply pdecompose'Eq in H0; subst; auto].
+  {inversion H; subst. 
+   {constructor; auto. apply pdecompose'Eq in H5; subst. auto. }
+   {constructor; auto. apply pdecompose'Eq in H6; subst; auto. }
+  }
+  {inversion H; subst; auto.  
+   {constructor; auto. apply pdecompose'Eq in H5; subst; auto. }
+   {constructor; auto. apply pdecompose'Eq in H6; subst; auto. }
+  }
+  {inversion H; subst; auto. constructor. apply IHt. auto. apply pdecompose'Eq in H2; subst; auto. }
+  {inversion H; subst; auto. constructor. apply IHt. auto. apply pdecompose'Eq in H2; subst; auto. }
+Qed. 
+
+Fixpoint pErase t :=
+  match t with
+    |pfvar i => pfvar' i
+    |pbvar i => pbvar' i
+    |punit => punit'
+    |ppair e1 e2 => ppair' (pErase e1) (pErase e2)
+    |plambda e => plambda' (pErase e)
+    |papp e1 e2 => papp' (pErase e1) (pErase e2)
+    |pret e => pret' (pErase e)
+    |pbind e1 e2 => pbind' (pErase e1) (pErase e2)
+    |pfork e => pfork' (pErase e)
+    |pnew => pnew'
+    |pput i e => pput' (pErase i) (pErase e)
+    |pget i => pget' (pErase i)
+    |praise e => praise' (pErase e)
+    |phandle e1 e2 => phandle' (pErase e1) (pErase e2)
+    |pfst e => pfst' (pErase e)
+    |psnd e => psnd' (pErase e)
+    |pdone e => pdone' (pErase e)
+    |pspec e1 e2 => pbind' (pErase e1) (plambda' (pbind' (pErase e2) (pret' (ppair' (pbvar' 0) (pbvar' 1)))))
+    |pspecRun e1 e2 => pbind' (pErase e1) (plambda' (pbind' (pErase e2) (pret' (ppair' (pbvar' 0) (pbvar' 1)))))
+    |pspecJoin e1 e2 => pbind' (pErase e1) (plambda' (pbind' (pErase e2) (pret' (ppair' (pbvar' 0) (pbvar' 1)))))
+  end. 
+
+Fixpoint pErasePool T :=
+  match T with
+      |t::ts => pErase t::pErasePool ts
+      |nil => nil
+  end. 
+
+Fixpoint raw_pEraseHeap (H: rawHeap pivar_state) :=
+  match H with
+      |(i, pempty)::H' => (i, pempty')::raw_pEraseHeap H'
+      |(i, pfull M)::H' => (i, pfull' (pErase M))::raw_pEraseHeap H'
+      |nil => nil
+  end. 
+
+Theorem pEraseHeapUnique : forall H S, 
+                             unique pivar_state S H ->
+                             unique pivar_state' S (raw_pEraseHeap H). 
+Proof.
+  induction H; intros. 
+  {constructor. }
+  {inv H0. simpl. destruct v; constructor; auto. }
+Qed. 
+
+Definition pEraseHeap H :=
+  match H with
+      |heap_ h p => heap_ pivar_state' (raw_pEraseHeap h) (pEraseHeapUnique h (Ensembles.Empty_set AST.id) p)
+  end. 
+
+Theorem ParImpliesPar' : forall H T t H' t', 
+                           pstep H T t (pOK H' T t') ->
+                           pstep' (pEraseHeap H) (pErasePool T) (pErasePool t)
+                                 (pOK' (pEraseHeap H') (pErasePool T) (pErasePool t')). 
+Admitted. 
+
+Require Import Spec. 
+
+Fixpoint specTerm' t :=
+  match t with
+    |pfvar' i => fvar i
+    |pbvar' i => bvar i
+    |punit' => unit
+    |ppair' e1 e2 => pair_ (specTerm' e1) (specTerm' e2)
+    |plambda' e => lambda (specTerm' e)
+    |papp' e1 e2 => app (specTerm' e1) (specTerm' e2)
+    |pret' e => ret (specTerm' e)
+    |pbind' e1 e2 => bind (specTerm' e1) (specTerm' e2)
+    |pfork' e => fork (specTerm' e)
+    |pnew' => new
+    |pput' i e => put (specTerm' i) (specTerm' e)
+    |pget' i => get (specTerm' i)
+    |praise' e => raise (specTerm' e)
+    |phandle' e1 e2 => handle (specTerm' e1) (specTerm' e2)
+    |pfst' e => fst (specTerm' e)
+    |psnd' e => snd (specTerm' e)
+    |pdone' e => done (specTerm' e)
+  end. 
+
+Inductive specPool' : pPool' -> pool -> Prop :=
+|specPool'Cons : forall t ts tid s2 Ts, 
+                   specPool' ts Ts ->
+                   specPool' (t::ts) ((tid,unlocked nil,s2,specTerm' t)::Ts)
+|specPoolNil' : specPool' nil nil. 
+
+Inductive raw_specHeap' : rawHeap pivar_state' -> rawHeap ivar_state -> Prop :=
+|specConsFull' : forall i tid M H H',
+                  raw_specHeap' H H' -> 
+                  raw_specHeap' ((i, pfull' M)::H) ((i, sfull COMMIT nil COMMIT tid (specTerm' M))::H')
+|specConsEmpty' : forall i H H', raw_specHeap' H H' -> 
+                                raw_specHeap'((i, pempty')::H) ((i, sempty COMMIT)::H')
+|specHeapNil' : raw_specHeap' nil nil. 
+
+Theorem spec'Unique : forall H S H',
+                       unique pivar_state' S H -> raw_specHeap' H H' ->
+                       unique ivar_state S H'. 
+Proof.
+  intros. Hint Constructors raw_specHeap'. generalize dependent S.
+  induction H1; intros. inv H0. constructor; auto. inv H0. constructor; auto. 
+  constructor. 
+Qed. 
+
+Inductive specHeap' : pHeap' -> sHeap -> Prop :=
+|specHeap_' : forall h h' proof (p':raw_specHeap' h h'), 
+               specHeap' (heap_ pivar_state' h proof)
+                        (heap_ ivar_state h' (spec'Unique h (Ensembles.Empty_set AST.id) h' proof p')). 
+
+Theorem Par'ImpliesSpec : forall H T t H' t' ST SH, 
+                            pstep' H T t (pOK' H' T t') -> specHeap' H SH ->
+                            specPool' (pUnion' T t) ST -> 
+                            exists SH' ST', multistep SH ST (Some(SH', ST')) /\
+                                            specPool' (pUnion' T t') ST' /\
+                                            specHeap' H' SH'. 
+Admitted. 
+
+
+Theorem ParImpliesSpec : forall H T t H' t' ST SH, 
+                            pstep H T t (pOK' H' T t') -> specHeap' H SH ->
+                            specPool (pUnion' T t) ST -> 
+                            exists SH' ST', multistep SH ST (Some(SH', ST')) /\
+                                            specPool' (pUnion' T t') ST' /\
+                                            specHeap' H' SH'. 
+Admitted. 
